Message reception formalized and Fake rule updated

scripts/DAP_Transaction.thy
@@ -10,13 +10,13 @@ begin
 inductive_set daptrans :: "event list set" where
   Nil: "[] \<in> daptrans"
 
-  | DT1: "\<lbrakk> evs1 \<in> daptrans \<rbrakk>
+  | DT1: "evs1 \<in> daptrans
     \<Longrightarrow> Says A Server \<lbrace> Agent A, Number T \<rbrace> # evs1 \<in> daptrans"
 
   | DT2: "\<lbrakk> evs2 \<in> daptrans;
           Says A' Server \<lbrace> Agent A, Number T \<rbrace> \<in> set evs2;
           Nonce r \<notin> used evs2;
-          r' = Crypt (shrK K) (Nonce r);
+          r' = Crypt (shrK A) (Nonce r);
           h_s = Hash \<lbrace> \<lbrace> Agent A, Number T \<rbrace>, r' \<rbrace> \<rbrakk>
     \<Longrightarrow> Says Server A \<lbrace> \<lbrace> Agent A, Number T \<rbrace>, r', h_s \<rbrace> # evs2 \<in> daptrans"
 
@@ -38,7 +38,7 @@ inductive_set daptrans :: "event list set" where
             Inputs A (Smartphone A) \<lbrace> Transaction, r', h_s \<rbrace> \<in> set evs5;
             Gets_a A Transaction' \<in> set evs5;
             Transaction == Transaction' \<rbrakk> 
-    \<Longrightarrow> Inputs A (Smartphone A) Confirmation # evs4 \<in> daptrans"
+    \<Longrightarrow> Inputs A (Smartphone A) Confirmation # evs5 \<in> daptrans"
 
   | DT6: "\<lbrakk> evs6 \<in> daptrans; 
             Gets_s (Smartphone A) \<lbrace> Transaction, r', h_s \<rbrace> \<in> set evs6;
@@ -47,7 +47,6 @@ inductive_set daptrans :: "event list set" where
             r_u \<notin> used evs6 \<rbrakk> 
    \<Longrightarrow> Outputs (Smartphone A) A r_u # evs6 \<in> daptrans"
 
-  (* TODO *)
   | DT7: "\<lbrakk> evs7 \<in> daptrans;
             Says A Server Transaction \<in> set evs7;
             Gets S \<lbrace> Transaction, r', h_u \<rbrace> \<in> set evs7; 
@@ -57,12 +56,24 @@ inductive_set daptrans :: "event list set" where
             Gets_a A r_u \<in> set evs7 \<rbrakk> 
     \<Longrightarrow> Says A Server r_u # evs7 \<in> daptrans"
 
-  | Fake: "\<lbrakk>evsf \<in> daptrans; X \<in> synth(analz(spies evsf))\<rbrakk> \<Longrightarrow> Says Spy B X # evsf \<in> daptrans"
+  | Fake: "\<lbrakk> evsf \<in> daptrans; X \<in> synth(analz(knows Spy evsf)) \<rbrakk> \<Longrightarrow> Says Spy B X # evsf \<in> daptrans"
+    
+  | Rcpt: "\<lbrakk> evsr \<in> daptrans; Says A B X \<in> set evsr \<rbrakk> \<Longrightarrow> Gets B X # evsr \<in> daptrans"
 
 
 lemma Protocol_terminates :
   "\<exists>r. \<exists>evs \<in> daptrans. Says A Server (Nonce r) \<in> set evs"
 apply (intro exI bexI)
-sorry
+apply (rule_tac [2] daptrans.DT7)
+apply (rule_tac [2] daptrans.DT6)
+apply (rule_tac [2] daptrans.DT5)
+apply (rule_tac [2] daptrans.DT4)
+apply (rule_tac [2] daptrans.DT3)
+apply (rule_tac [2] daptrans.DT2)
+apply (rule_tac [2] daptrans.DT1)
+apply (rule_tac [2] daptrans.Nil)
+apply (possibility)
+apply (auto)
+done
 
 end
